work on temporal_deep example
Following some work by Chun Tian, this commit makes the temporal_deep
example compile again. This example got severe bit-rot unluckily. There
is still more work to do:

- the libraries have not been tested yet
- the theories contaimn now many constants and lemmata now present in
standard libraries
- the proofs are ugly using strange constructs which are hard to
maintain (I hope I learned something about HOL within the last 10 years
since I created this example)

So, this commit is just a first step and more cleanup work will follow.

examples/temporal_deep/src/tools/tuerk_tacticsLib.sml
@@ -142,8 +142,8 @@ struct
    val IMP_TAC = fn t => ASSUME_TAC t THEN UNDISCH_HD_TAC;
    fun GSYM_NO_TAC i = POP_NO_ASSUM i (fn x=> ASSUME_TAC (GSYM x));
 
-   val SUBGOAL_TAC = (fn t => (t by ALL_TAC));
-   val REMAINS_TAC = (fn t => (Tactical.REVERSE(t by ALL_TAC)));
+   fun SUBGOAL_TAC q = Q.SUBGOAL_THEN q STRIP_ASSUME_TAC
+   fun REMAINS_TAC q = Tactical.REVERSE (SUBGOAL_TAC q)
    val SPEC_NO_ASSUM = (fn n => fn S => POP_NO_ASSUM n (fn x=> ASSUME_TAC (SPEC S x)));
    val SPECL_NO_ASSUM = (fn n => fn S => POP_NO_ASSUM n (fn x=> ASSUME_TAC (SPECL S x)));
 
