examples/temporal_deep/src/deep_embeddings/rltlScript.sml
@@ -3,9 +3,9 @@ open HolKernel Parse boolLib bossLib;
 (*
 quietdec := true;
 
-val home_dir = (concat Globals.HOLDIR "/examples/temporal_deep/");
-loadPath := (concat home_dir "src/deep_embeddings") ::
-            (concat home_dir "src/tools") :: !loadPath;
+val home_dir = (Globals.HOLDIR ^ "/examples/temporal_deep/");
+loadPath := (home_dir ^ "src/deep_embeddings") ::
+            (home_dir ^ "src/tools") :: !loadPath;
 
 map load
  ["infinite_pathTheory", "prop_logicTheory", "pred_setTheory", "arithmeticTheory", "tuerk_tacticsLib", "numLib", "symbolic_kripke_structureTheory", "set_lemmataTheory"];
@@ -27,6 +27,8 @@ val _ = hide "I";
 
 val _ = new_theory "rltl";
 
+val Know = Q_TAC KNOW_TAC;
+val Suff = Q_TAC SUFF_TAC;
 
 (******************************************************************************
 * Syntax and semantic
@@ -54,7 +56,7 @@ val rltl_induct =
         PROVE[]``(!x y. P x ==> Q(x,y)) = !x. P x ==> !y. Q(x,y)``,
         PROVE[]``(!x y. P y ==> Q(x,y)) = !y. P y ==> !x. Q(x,y)``]
        (Q.SPECL
-         [`P`,`\(f1,f2). P f1 /\ P f2`, `\(f,b). P f`]
+         [`P`,`\(f,b). P f`,`\(f1,f2). P f1 /\ P f2`]
          (TypeBase.induction_of ``:'a rltl``)))));
 
 
@@ -803,26 +805,26 @@ val RLTL_EQUIV_PATH_STRONG_THM =
       REWRITE_TAC [RLTL_SEM_TIME_def] THEN
       METIS_TAC [RLTL_EQUIV_PATH_STRONG___SUC, RLTL_EQUIV_PATH_STRONG___INITIAL],
 
-      REMAINS_TAC `!v1 v2. RLTL_EQUIV_PATH_STRONG t v1 v2 a r /\ RLTL_SEM_TIME t v1 a r (RLTL_SUNTIL (f,f')) ==> RLTL_SEM_TIME t v2 a r (RLTL_SUNTIL (f,f'))` THEN1 (
+      Suff `!v1 v2. RLTL_EQUIV_PATH_STRONG t v1 v2 a r /\ RLTL_SEM_TIME t v1 a r (RLTL_SUNTIL (f,f')) ==> RLTL_SEM_TIME t v2 a r (RLTL_SUNTIL (f,f'))` THEN1 (
         METIS_TAC[RLTL_EQUIV_PATH_STRONG___SYM_PATH]
       ) THEN
       WEAKEN_HD_TAC THEN
       SIMP_TAC arith_ss [RLTL_EQUIV_PATH_STRONG_def, RLTL_SEM_TIME_def] THEN
       REPEAT STRIP_TAC THEN (
         `?l. MIN k k' = l` by METIS_TAC[] THEN
-        SUBGOAL_TAC `l <= k /\ l <= k' /\ l >= t` THEN1 (
+        Know `l <= k /\ l <= k' /\ l >= t` THEN1 (
           REWRITE_TAC[GSYM (ASSUME ``MIN k k' = l``), MIN_DEF] THEN
           Cases_on `k < k'` THEN
           ASM_REWRITE_TAC[] THEN
           DECIDE_TAC
-        ) THEN
-        SUBGOAL_TAC `!j. (t <= j /\ j <= l) ==> (RLTL_EQUIV_PATH_STRONG j v1 v2 a r)` THEN1 (
+        ) THEN DISCH_TAC THEN
+        Know `!j. (t <= j /\ j <= l) ==> (RLTL_EQUIV_PATH_STRONG j v1 v2 a r)` THEN1 (
               REWRITE_TAC[RLTL_EQUIV_PATH_STRONG_def] THEN
               REPEAT STRIP_TAC THEN
               `k >= j /\ !j':num. (j <= j') ==> (t <= j')` by DECIDE_TAC THEN
               EXISTS_TAC ``k:num`` THEN
               METIS_TAC[]
-        ) THEN
+        ) THEN DISCH_TAC THEN
         EXISTS_TAC ``l:num`` THEN
         `l >= t` by DECIDE_TAC THEN
         ASM_REWRITE_TAC [] THEN
@@ -847,7 +849,7 @@ val RLTL_EQUIV_PATH_STRONG_THM =
 
 
       SIMP_TAC std_ss [RLTL_SEM_TIME_def] THEN
-      SUBGOAL_TAC `RLTL_EQUIV_PATH_STRONG t v1 v2 (P_OR (a,P_AND (p_2,P_NOT r))) r` THEN1 (
+      Know `RLTL_EQUIV_PATH_STRONG t v1 v2 (P_OR (a,P_AND (p_2,P_NOT r))) r` THEN1 (
          REWRITE_ALL_TAC[RLTL_EQUIV_PATH_STRONG_def, P_SEM_THM] THEN
          EXISTS_TAC ``k:num`` THEN
          ASM_REWRITE_TAC[]
@@ -885,28 +887,28 @@ val RLTL_SEM_TIME___ACCEPT_BEFORE_ON_PATH =
       METIS_TAC[RLTL_SEM_TIME___ACCEPT_REJECT_IMP_ON_PATH],
 
 
-      SUBGOAL_TAC `?u. (t <= u /\ P_SEM (v u) a1) /\ (!u'. (t <= u' /\ u' < u) ==>
+      Know `?u. (t <= u /\ P_SEM (v u) a1) /\ (!u'. (t <= u' /\ u' < u) ==>
          (~P_SEM (v u') a1) /\ ~P_SEM (v u') a2)` THEN1 (
 
          SIMP_ALL_TAC std_ss [NOT_ON_PATH_RESTN_def] THEN
-         SUBGOAL_TAC `?k. (P_SEM (v k) a2 /\ t <= k) /\ !k'. (t <= k' /\ k' < k) ==> ~(P_SEM (v k') a2)` THEN1 (
+         Know `?k. (P_SEM (v k) a2 /\ t <= k) /\ !k'. (t <= k' /\ k' < k) ==> ~(P_SEM (v k') a2)` THEN1 (
             ASSUME_TAC (EXISTS_LEAST_CONV ``?k. (P_SEM (v k) a2) /\  t <= k``) THEN
             METIS_TAC[]
-         ) THEN
+         ) THEN DISCH_TAC THEN
          REWRITE_ALL_TAC [BEFORE_ON_PATH_RESTN_def] THEN
          `?k'. t <= k' /\ k' <= k /\ P_SEM (v k') a1` by METIS_TAC[] THEN
 
-         SUBGOAL_TAC `?u. (P_SEM (v u) a1 /\ t <= u) /\ !l'. (t <= l' /\ l' < u) ==> ~(P_SEM (v l') a1)` THEN1 (
+         Know `?u. (P_SEM (v u) a1 /\ t <= u) /\ !l'. (t <= l' /\ l' < u) ==> ~(P_SEM (v l') a1)` THEN1 (
             ASSUME_TAC (EXISTS_LEAST_CONV ``?u. (P_SEM (v u) a1) /\  t <= u``) THEN
             METIS_TAC[]
-         ) THEN
+         ) THEN STRIP_TAC THEN
 
          EXISTS_TAC ``u:num`` THEN
          ASM_REWRITE_TAC[] THEN
          `~(k' < u)` by METIS_TAC[] THEN
          `!u'. u' < u ==> u' < k` by DECIDE_TAC THEN
          METIS_TAC[]
-      ) THEN
+      ) THEN STRIP_TAC THEN
 
 
 
@@ -919,13 +921,13 @@ val RLTL_SEM_TIME___ACCEPT_BEFORE_ON_PATH =
 
 
       SUBGOAL_THEN ``RLTL_SEM_TIME t v (P_OR(a1, a2)) r f`` STRIP_ASSUME_TAC THEN1 (
-         SUBGOAL_TAC `IMP_ON_PATH_RESTN t v a2 (P_OR (a1,a2))` THEN1 (
+         Know `IMP_ON_PATH_RESTN t v a2 (P_OR (a1,a2))` THEN1 (
            SIMP_TAC std_ss [IMP_ON_PATH_RESTN_def, P_SEM_THM]
          ) THEN
          METIS_TAC[RLTL_SEM_TIME___ACCEPT_REJECT_IMP_ON_PATH]
       ) THEN
 
-      SUBGOAL_TAC `(RLTL_EQUIV_PATH_STRONG t v w a1 r) /\ (RLTL_EQUIV_PATH_STRONG t v w (P_OR(a1, a2)) r)` THEN1 (
+      Know `(RLTL_EQUIV_PATH_STRONG t v w a1 r) /\ (RLTL_EQUIV_PATH_STRONG t v w (P_OR(a1, a2)) r)` THEN1 (
          REWRITE_TAC[RLTL_EQUIV_PATH_STRONG_def, GREATER_EQ, P_SEM_THM] THEN
          REPEAT STRIP_TAC THEN
          EXISTS_TAC ``u:num`` THEN
@@ -934,9 +936,9 @@ val RLTL_SEM_TIME___ACCEPT_BEFORE_ON_PATH =
          REPEAT STRIP_TAC THEN
          `~(u < l)` by DECIDE_TAC THEN
          METIS_TAC[]
-      ) THEN
+      ) THEN DISCH_TAC THEN
 
-      SUBGOAL_TAC `IMP_ON_PATH_RESTN t w (P_OR(a1,a2)) a1` THEN1 (
+      Know `IMP_ON_PATH_RESTN t w (P_OR(a1,a2)) a1` THEN1 (
          REWRITE_TAC [IMP_ON_PATH_RESTN_def, GREATER_EQ, P_SEM_THM] THEN
          REPEAT STRIP_TAC THEN
          Cases_on `u < t'` THENL [
@@ -950,7 +952,7 @@ val RLTL_SEM_TIME___ACCEPT_BEFORE_ON_PATH =
                `t' < u` by DECIDE_TAC THEN
                METIS_TAC[]
             ]
-         ]) THEN
+         ]) THEN DISCH_TAC THEN
 
       PROVE_TAC[RLTL_EQUIV_PATH_STRONG_THM, RLTL_SEM_TIME___ACCEPT_REJECT_IMP_ON_PATH]
    ]);
@@ -978,13 +980,13 @@ val RLTL_SEM_TIME___ACCEPT_OR_THM =
    REPEAT STRIP_TAC THEN
    EQ_TAC THENL [
       DISJ_CASES_TAC (SPECL [``v:num->'a set``, ``t:num``, ``a1:'a prop_logic``, ``a2:'a prop_logic``] BEFORE_ON_PATH_CASES) THENL [
-         SUBGOAL_TAC `BEFORE_ON_PATH_RESTN t v a1 (P_OR (a1,a2))` THEN1 (
+         Know `BEFORE_ON_PATH_RESTN t v a1 (P_OR (a1,a2))` THEN1 (
             REWRITE_ALL_TAC [BEFORE_ON_PATH_RESTN_def, P_SEM_THM] THEN
             PROVE_TAC[LESS_EQ_REFL]
          ) THEN
          PROVE_TAC[RLTL_SEM_TIME___ACCEPT_BEFORE_ON_PATH],
 
-         SUBGOAL_TAC `BEFORE_ON_PATH_RESTN t v a2 (P_OR (a1,a2))` THEN1 (
+         Know `BEFORE_ON_PATH_RESTN t v a2 (P_OR (a1,a2))` THEN1 (
             REWRITE_ALL_TAC [BEFORE_ON_PATH_RESTN_def, P_SEM_THM] THEN
             PROVE_TAC[LESS_EQ_REFL]
          ) THEN
@@ -1084,12 +1086,12 @@ val RLTL_WEAK_UNTIL___ALTERNATIVE_DEF =
 
          DISJ1_TAC THEN
          SIMP_ASSUMPTIONS_TAC std_ss [] THEN
-         SUBGOAL_TAC `?k. (k >= (t:num) /\ ~RLTL_SEM_TIME k v a r f1) /\ !k'. k' < k ==> ~(k' >= t /\ ~RLTL_SEM_TIME k' v a r f1)` THEN1 (
+         Know `?k. (k >= (t:num) /\ ~RLTL_SEM_TIME k v a r f1) /\ !k'. k' < k ==> ~(k' >= t /\ ~RLTL_SEM_TIME k' v a r f1)` THEN1 (
             ASSUME_TAC (EXISTS_LEAST_CONV ``?k. k >= (t:num) /\ ~RLTL_SEM_TIME k (v:num -> 'a set) a r f1``) THEN
             RES_TAC THEN
             PROVE_TAC[]
-         ) THEN
-         SUBGOAL_TAC `?l:num. l >= (t:num) /\ l <= (k':num) /\ RLTL_SEM_TIME l v a r f2` THEN1 (
+         ) THEN STRIP_TAC THEN
+         Know `?l:num. l >= (t:num) /\ l <= (k':num) /\ RLTL_SEM_TIME l v a r f2` THEN1 (
             Cases_on `RLTL_SEM_TIME k' v a r f2` THENL [
                EXISTS_TAC ``k':num`` THEN
                ASM_SIMP_TAC arith_ss [],
@@ -1098,7 +1100,7 @@ val RLTL_WEAK_UNTIL___ALTERNATIVE_DEF =
                EXISTS_TAC ``j:num`` THEN
                ASM_SIMP_TAC arith_ss []
             ]
-         ) THEN
+         ) THEN STRIP_TAC THEN
          EXISTS_TAC ``l:num`` THEN
          ASM_SIMP_TAC arith_ss [] THEN
          REPEAT STRIP_TAC THEN
@@ -1168,14 +1170,14 @@ val RLTL_SEM_TIME___VAR_RENAMING =
         RLTL_VAR_RENAMING_def, PATH_VAR_RENAMING_def,
         PATH_MAP_def] THEN
       REPEAT STRIP_TAC THEN
-      REMAINS_TAC `INJ f ((v t) UNION P_USED_VARS a) UNIV /\
+      Suff `INJ f ((v t) UNION P_USED_VARS a) UNIV /\
                    INJ f ((v t) UNION P_USED_VARS p) UNIV /\
                    INJ f ((v t) UNION P_USED_VARS r) UNIV` THEN1 (
         ASM_SIMP_TAC std_ss [GSYM P_SEM___VAR_RENAMING]
-      ) THEN
+      ) THEN STRIP_TAC THEN
       REPEAT STRIP_TAC THEN
       UNDISCH_HD_TAC THEN
-      MATCH_MP_TAC INJ_SUBSET THEN
+      MATCH_MP_TAC INJ_SUBSET_DOMAIN THEN
       REWRITE_TAC [SUBSET_DEF, IN_UNION, RLTL_USED_VARS_def,
         GSYM PATH_USED_VARS_THM] THEN
       PROVE_TAC[],
@@ -1191,17 +1193,18 @@ val RLTL_SEM_TIME___VAR_RENAMING =
       SIMP_TAC std_ss [RLTL_SEM_TIME_def, RLTL_USED_VARS_def,
         RLTL_VAR_RENAMING_def] THEN
       REPEAT STRIP_TAC THEN
-      REMAINS_TAC `INJ f (PATH_USED_VARS v UNION RLTL_USED_VARS f'' UNION
+      Suff `INJ f (PATH_USED_VARS v UNION RLTL_USED_VARS f'' UNION
                           P_USED_VARS a UNION P_USED_VARS r) UNIV /\
                    INJ f (PATH_USED_VARS v UNION RLTL_USED_VARS f' UNION
                           P_USED_VARS a UNION P_USED_VARS r) UNIV` THEN1 (
+        STRIP_TAC THEN
         RES_TAC THEN
         ASM_REWRITE_TAC[]
-      ) THEN
+      ) THEN 
       NTAC 2 (WEAKEN_NO_TAC 1) THEN
       STRIP_TAC THEN
       UNDISCH_HD_TAC THEN
-      MATCH_MP_TAC INJ_SUBSET THEN
+      MATCH_MP_TAC INJ_SUBSET_DOMAIN THEN
       SIMP_TAC std_ss [SUBSET_DEF, IN_UNION] THEN
       PROVE_TAC[],
 
@@ -1213,13 +1216,13 @@ val RLTL_SEM_TIME___VAR_RENAMING =
       UNDISCH_HD_TAC THEN ASM_REWRITE_TAC[] THEN STRIP_TAC THEN
       ASM_REWRITE_TAC[] THEN
       WEAKEN_HD_TAC THEN
-      REMAINS_TAC `INJ f ((v t) UNION P_USED_VARS a) UNIV /\
+      Suff `INJ f ((v t) UNION P_USED_VARS a) UNIV /\
                    INJ f ((v t) UNION P_USED_VARS r) UNIV` THEN1 (
         ASM_SIMP_TAC std_ss [GSYM P_SEM___VAR_RENAMING, PATH_VAR_RENAMING_def,
           PATH_MAP_def]
       ) THEN
       STRIP_TAC THEN UNDISCH_HD_TAC THEN
-      MATCH_MP_TAC INJ_SUBSET THEN
+      MATCH_MP_TAC INJ_SUBSET_DOMAIN THEN
       SIMP_TAC std_ss [SUBSET_DEF, IN_UNION, GSYM PATH_USED_VARS_THM] THEN
       PROVE_TAC[],
 
@@ -1227,17 +1230,18 @@ val RLTL_SEM_TIME___VAR_RENAMING =
       SIMP_TAC std_ss [RLTL_SEM_TIME_def, RLTL_USED_VARS_def,
         RLTL_VAR_RENAMING_def] THEN
       REPEAT STRIP_TAC THEN
-      REMAINS_TAC `INJ f (PATH_USED_VARS v UNION RLTL_USED_VARS f'' UNION
+      Suff `INJ f (PATH_USED_VARS v UNION RLTL_USED_VARS f'' UNION
                           P_USED_VARS a UNION P_USED_VARS r) UNIV /\
                    INJ f (PATH_USED_VARS v UNION RLTL_USED_VARS f' UNION
                           P_USED_VARS a UNION P_USED_VARS r) UNIV` THEN1 (
+        STRIP_TAC THEN
         RES_TAC THEN
         ASM_REWRITE_TAC[]
       ) THEN
       NTAC 2 (WEAKEN_NO_TAC 1) THEN
       STRIP_TAC THEN
       UNDISCH_HD_TAC THEN
-      MATCH_MP_TAC INJ_SUBSET THEN
+      MATCH_MP_TAC INJ_SUBSET_DOMAIN THEN
       SIMP_TAC std_ss [SUBSET_DEF, IN_UNION] THEN
       PROVE_TAC[],
 
@@ -1246,13 +1250,14 @@ val RLTL_SEM_TIME___VAR_RENAMING =
       SIMP_TAC std_ss [RLTL_SEM_TIME_def, RLTL_USED_VARS_def,
         RLTL_VAR_RENAMING_def, GSYM P_VAR_RENAMING_def, P_OR_def] THEN
       REPEAT STRIP_TAC THEN
-      REMAINS_TAC `INJ f (PATH_USED_VARS v UNION RLTL_USED_VARS f' UNION
+      Suff `INJ f (PATH_USED_VARS v UNION RLTL_USED_VARS f' UNION
                           P_USED_VARS (P_NOT (P_AND (P_NOT a,P_NOT (P_AND (p_2,P_NOT r))))) UNION P_USED_VARS r) UNIV` THEN1 (
+        STRIP_TAC THEN
         RES_TAC THEN
         ASM_REWRITE_TAC[]
       ) THEN
       UNDISCH_HD_TAC THEN
-      MATCH_MP_TAC INJ_SUBSET THEN
+      MATCH_MP_TAC INJ_SUBSET_DOMAIN THEN
       SIMP_TAC std_ss [SUBSET_DEF, IN_UNION, P_USED_VARS_def] THEN
       PROVE_TAC[]
    ]);
@@ -1270,7 +1275,7 @@ val RLTL_SEM_TIME___VAR_RENAMING___PATH_RESTRICT =
    CONV_TAC (LHS_CONV (ONCE_REWRITE_CONV [RLTL_USED_VARS_INTER_THM])) THEN
    MATCH_MP_TAC RLTL_SEM_TIME___VAR_RENAMING THEN
    UNDISCH_HD_TAC THEN
-   MATCH_MP_TAC INJ_SUBSET THEN
+   MATCH_MP_TAC INJ_SUBSET_DOMAIN THEN
    SIMP_TAC std_ss [SUBSET_DEF, IN_UNION, GSYM PATH_USED_VARS_THM,
     PATH_RESTRICT_def, PATH_MAP_def, IN_INTER] THEN
    PROVE_TAC[]);
@@ -1284,7 +1289,7 @@ val RLTL_SEM___VAR_RENAMING___PATH_RESTRICT =
 
    REPEAT STRIP_TAC THEN
    REWRITE_TAC[RLTL_SEM_def] THEN
-   SUBGOAL_TAC `P_FALSE = P_VAR_RENAMING f P_FALSE` THEN1 (
+   Know `P_FALSE = P_VAR_RENAMING f P_FALSE` THEN1 (
       SIMP_TAC std_ss [P_FALSE_def, P_VAR_RENAMING_def]
    ) THEN
    ASM_REWRITE_TAC[] THEN
